src/model/thread_info.v
@@ -1,13 +1,47 @@
+From Coq Require Import Lists.List.
+From Coq Require Import micromega.Lia.
 From Coq Require Import ZArith.ZArith.
 
 From compcert Require Import common.Values.
 
+From VST Require Import floyd.sublist.
+From VST Require Import msl.Coqlib2.
+
 From CertiGC Require Import model.constants.
+From CertiGC Require Import model.graph.
 From CertiGC Require Import model.heap.
+
 
 Record thread_info: Type := {
     ti_heap_p: val;
     ti_heap: Heap;
     ti_args: list val;
     arg_size: Zlength ti_args = MAX_ARGS;
+}.
+
+Definition nth_space (t_info: thread_info) (n: nat): Space :=
+  nth n t_info.(ti_heap).(heap_spaces) null_space.
+
+Lemma nth_space_Znth: forall t n,
+    nth_space t n = Znth (Z.of_nat n) (heap_spaces (ti_heap t)).
+Proof.
+  intros. unfold nth_space, Znth. rewrite if_false. 2: lia.
+  rewrite Nat2Z.id. reflexivity.
+Qed.
+
+Definition gen_size t_info n := space_capacity (nth_space t_info n).
+
+Definition rest_gen_size (t_info: thread_info) (gen: nat): Z :=
+  space_capacity (nth_space t_info gen) - space_allocated (nth_space t_info gen).
+
+Definition enough_space_to_copy g t_info from to: Prop :=
+  (unmarked_gen_size g from <= rest_gen_size t_info to)%Z.
+
+
+Record fun_info : Type := {
+    fun_word_size: Z;
+    live_roots_indices: list Z;
+    fi_index_range: forall i, In i live_roots_indices -> (0 <= i < MAX_ARGS)%Z;
+    lri_range: (Zlength (live_roots_indices) <= MAX_UINT - 2)%Z;
+    word_size_range: (0 <= fun_word_size <= MAX_UINT)%Z;
 }.
