src/model/compatible.v
@@ -1,0 +1,168 @@
+From Coq Require Import Lists.List.
+
+From VST Require Import floyd.sublist.
+From VST Require Import veric.base.
+
+From CertiGraph Require Import graph.graph_model.
+From CertiGraph Require Import lib.List_ext.
+
+From CertiGC Require Import model.constants.
+From CertiGC Require Import model.graph.
+From CertiGC Require Import model.heap.
+From CertiGC Require Import model.thread_info.
+From CertiGC Require Import model.util.
+
+
+Definition roots_outlier_compatible (roots: roots_t) (outlier: outlier_t): Prop :=
+  incl (filter_sum_right (filter_sum_left roots)) outlier.
+
+Definition roots_graph_compatible (roots: roots_t) (g: HeapGraph): Prop :=
+  Forall (graph_has_v g) (filter_sum_right roots).
+
+Definition roots_compatible (g: HeapGraph) (outlier: outlier_t) (roots: roots_t): Prop :=
+  roots_outlier_compatible roots outlier /\ roots_graph_compatible roots g.
+
+
+Definition outlier_compatible (g: HeapGraph) (outlier: outlier_t): Prop :=
+  forall v,
+    graph_has_v g v ->
+    incl (filter_sum_right (filter_option (vlabel g v).(block_fields))) outlier.
+
+Lemma in_gcptr_outlier: forall g gcptr outlier n v,
+    graph_has_v g v ->
+    outlier_compatible g outlier ->
+    0 <= n < Zlength (block_fields (vlabel g v)) ->
+    Znth n (make_fields g v) = inl (inr gcptr) ->
+    In gcptr outlier.
+Proof.
+  intros.
+  apply H0 in H; apply H; clear H; clear H0.
+  unfold make_fields in H2.
+  apply make_fields'_item_was_in_list in H2; try assumption.
+  rewrite <- filter_sum_right_In_iff, <- filter_option_In_iff.
+  rewrite <- H2; apply Znth_In; assumption.
+Qed.
+
+
+Definition generation_space_compatible (g: HeapGraph)
+           (tri: nat * Generation * Space) : Prop :=
+  match tri with
+  | (gen, gi, sp) =>
+    generation_base gi = sp.(space_base) /\
+    generation_sh gi = sp.(space_sh) /\
+    previous_vertices_size g gen gi.(generation_block_count) = sp.(space_allocated)
+  end.
+
+Definition graph_thread_info_compatible (g: HeapGraph) (ti: thread_info): Prop :=
+  Forall (generation_space_compatible g)
+         (combine (combine (nat_inc_list (length g.(glabel).(generations)))
+                           g.(glabel).(generations)) ti.(ti_heap).(heap_spaces)) /\
+  Forall (eq nullval)
+         (skipn (length g.(glabel).(generations)) (map space_base ti.(ti_heap).(heap_spaces))) /\
+  (length g.(glabel).(generations) <= length ti.(ti_heap).(heap_spaces))%nat.
+
+Definition fun_thread_arg_compatible
+           (g: HeapGraph) (ti: thread_info) (fi: fun_info) (roots: roots_t) : Prop :=
+  map (root2val g) roots = map ((fun x y => Znth y x) ti.(ti_args)) fi.(live_roots_indices).
+
+
+Definition copy_compatible (g: HeapGraph): Prop :=
+  forall v, graph_has_v g v -> (vlabel g v).(block_mark) = true ->
+            graph_has_v g (vlabel g v).(block_copied_vertex) /\
+            addr_gen v <> addr_gen (vlabel g v).(block_copied_vertex).
+
+
+Definition super_compatible (g_ti_r: HeapGraph * thread_info * roots_t) (fi: fun_info) (out: outlier_t) : Prop
+ := let (g_ti, r) := g_ti_r
+ in let (g, ti) := g_ti
+ in graph_thread_info_compatible g ti /\
+    fun_thread_arg_compatible g ti fi r /\
+    roots_compatible g out r /\
+    outlier_compatible g out.
+
+
+Lemma gsc_iff: forall (g: HeapGraph) t_info,
+    (length (generations (glabel g)) <= length (heap_spaces (ti_heap t_info)))%nat ->
+    Forall (generation_space_compatible g)
+           (combine (combine (nat_inc_list (length (generations (glabel g))))
+                             (generations (glabel g))) (heap_spaces (ti_heap t_info))) <->
+    forall gen,
+      graph_has_gen g gen ->
+      generation_space_compatible g (gen, nth_gen g gen, nth_space t_info gen).
+Proof.
+  intros. rewrite Forall_forall. remember (generations (glabel g)).
+  remember (nat_inc_list (length l)). remember (heap_spaces (ti_heap t_info)).
+  assert (length (combine l0 l) = length l) by
+      (subst; rewrite combine_length, nat_inc_list_length, Nat.min_id; reflexivity).
+  assert (length (combine (combine l0 l) l1) = length l) by
+      (rewrite combine_length, H0, min_l by assumption; reflexivity).
+  cut (forall x, In x (combine (combine l0 l) l1) <->
+                    exists gen, graph_has_gen g gen /\
+                                x = (gen, nth_gen g gen, nth_space t_info gen)).
+  - intros. split; intros.
+    + apply H3. rewrite H2. exists gen. intuition.
+    + rewrite H2 in H4. destruct H4 as [gen [? ?]]. subst x. apply H3. assumption.
+  - intros.
+    assert (forall gen,
+               graph_has_gen g gen ->
+               nth gen (combine (combine l0 l) l1) (O, null_generation, null_space) =
+               (gen, nth_gen g gen, nth_space t_info gen)). {
+      intros. red in H2. rewrite <- Heql in H2.
+      rewrite combine_nth_lt; [|rewrite H0; lia | lia].
+      rewrite combine_nth by (subst l0; rewrite nat_inc_list_length; reflexivity).
+      rewrite Heql0. rewrite nat_inc_list_nth by assumption.
+      rewrite Heql. unfold nth_gen, nth_space. rewrite Heql1. reflexivity. }
+    split; intros.
+    + apply (In_nth (combine (combine l0 l) l1) x (O, null_generation, null_space)) in H3.
+      destruct H3 as [gen [? ?]]. exists gen. rewrite H1 in H3.
+      assert (graph_has_gen g gen) by (subst l; assumption). split. 1: assumption.
+      rewrite H2 in H4 by assumption. subst x. reflexivity.
+    + destruct H3 as [gen [? ?]]. rewrite <- H2 in H4 by assumption. subst x.
+      apply nth_In. rewrite H1. subst l. assumption.
+Qed.
+
+Lemma gt_gs_compatible:
+  forall (g: HeapGraph) (t_info: thread_info),
+    graph_thread_info_compatible g t_info ->
+    forall gen,
+      graph_has_gen g gen ->
+      generation_space_compatible g (gen, nth_gen g gen, nth_space t_info gen).
+Proof.
+  intros. destruct H as [? [_ ?]]. rewrite gsc_iff in H by assumption.
+  apply H. assumption.
+Qed.
+
+
+Definition forward_roots_compatible
+           (from to: nat) (g: HeapGraph) (ti : thread_info): Prop :=
+  (nth_space ti from).(space_allocated) <= (nth_space ti to).(space_capacity) -
+                                      (nth_space ti to).(space_allocated).
+
+
+
+Lemma graph_thread_v_in_range (g: HeapGraph) (t_info: thread_info) (v: Addr)
+    (Hcompat: graph_thread_info_compatible g t_info)
+    (Hv: graph_has_v g v):
+    v_in_range
+        (vertex_address g v)
+        (gen_start g (addr_gen v))
+        (WORD_SIZE * gen_size t_info (addr_gen v)).
+Proof.
+    exists (WORD_SIZE * vertex_offset g v).
+    pose proof WORD_SIZE_pos as HH.
+    repeat split.
+    {
+        pose proof (previous_vertices_size__nonneg g (addr_gen v) (addr_block v)) as HH'.
+        unfold vertex_offset.
+        lia.
+    }
+    {
+        apply Zmult_lt_compat_l ; try assumption.
+        pose proof (proj2 (space__order (nth_space t_info (addr_gen v)))) as HH'.
+        apply Z.lt_le_trans with (space_allocated (nth_space t_info (addr_gen v))) ; try assumption.
+        destruct Hv as [Hv_gen Hv_index].
+        destruct (gt_gs_compatible _ _ Hcompat _ Hv_gen) as [Estart [Esh Eused]].
+        rewrite <- Eused.
+        now apply vo_lt_gs.
+    }
+Qed.
