src/model/forward.v
@@ -1,0 +1,348 @@
+From Coq Require Import Lists.List.
+From Coq Require Import micromega.Lia.
+From Coq Require Import ZArith.ZArith.
+
+From compcert Require Import common.Values.
+From compcert Require Import lib.Integers.
+
+From VST Require Import floyd.functional_base.
+From VST Require Import floyd.sublist.
+From VST Require Import msl.shares.
+From VST Require Import veric.base.
+From VST Require Import veric.shares.
+From VST Require Import veric.val_lemmas.
+
+From CertiGraph Require Export graph.graph_gen.
+From CertiGraph Require Import graph.graph_model.
+From CertiGraph Require Import lib.EquivDec_ext.
+From CertiGraph Require Import lib.List_ext.
+
+From CertiGC Require Import model.copy.
+From CertiGC Require Import model.compatible.
+From CertiGC Require Import model.constants.
+From CertiGC Require Import model.graph.
+From CertiGC Require Import model.heap.
+From CertiGC Require Import model.thread_info.
+From CertiGC Require Import model.update.
+From CertiGC Require Import model.util.
+
+Local Coercion pg_lg: LabeledGraph >-> PreGraph.
+
+
+Definition forward_t: Type := Z + GC_Pointer + Addr + Field.
+
+Definition root2forward (r: root_t): forward_t :=
+  match r with
+  | inl (inl z) => inl (inl (inl z))
+  | inl (inr p) => inl (inl (inr p))
+  | inr v => inl (inr v)
+  end.
+
+Definition field2forward (f: field_t): forward_t :=
+  match f with
+  | inl (inl z) => inl (inl (inl z))
+  | inl (inr p) => inl (inl (inr p))
+  | inr e => inr e
+  end.
+
+Definition forward_p_type: Type := Z + (Addr * Z).
+
+Definition forward_p2forward_t
+           (p: forward_p_type) (roots: roots_t) (g: HeapGraph): forward_t :=
+  match p with
+  | inl root_index => root2forward (Znth root_index roots)
+  | inr (v, n) => if (vlabel g v).(block_mark) && (n =? 0)
+                  then (inl (inr (vlabel g v).(block_copied_vertex)))
+                  else field2forward (Znth n (make_fields g v))
+  end.
+
+Definition vertex_pos_pairs (g: HeapGraph) (v: Addr) : list (forward_p_type) :=
+  map (fun x => inr (v, Z.of_nat x))
+      (nat_inc_list (length (block_fields (vlabel g v)))).
+
+Inductive forward_relation (from to: nat):
+  nat -> forward_t -> HeapGraph -> HeapGraph -> Prop :=
+| fr_z: forall depth z g, forward_relation from to depth (inl (inl (inl z))) g g
+| fr_p: forall depth p g, forward_relation from to depth (inl (inl (inr p))) g g
+| fr_v_not_in: forall depth v g,
+    addr_gen v <> from -> forward_relation from to depth (inl (inr v)) g g
+| fr_v_in_forwarded: forall depth v g,
+    addr_gen v = from -> (vlabel g v).(block_mark) = true ->
+    forward_relation from to depth (inl (inr v)) g g
+| fr_v_in_not_forwarded_O: forall v g,
+    addr_gen v = from -> (vlabel g v).(block_mark) = false ->
+    forward_relation from to O (inl (inr v)) g (lgraph_copy_v g v to)
+| fr_v_in_not_forwarded_Sn: forall depth v g g',
+    addr_gen v = from -> (vlabel g v).(block_mark) = false ->
+    let new_g := lgraph_copy_v g v to in
+    forward_loop from to depth (vertex_pos_pairs new_g (new_copied_v g to)) new_g g' ->
+    forward_relation from to (S depth) (inl (inr v)) g g'
+| fr_e_not_to: forall depth e (g: HeapGraph),
+    addr_gen (dst g e) <> from -> forward_relation from to depth (inr e) g g
+| fr_e_to_forwarded: forall depth e (g: HeapGraph),
+    addr_gen (dst g e) = from -> (vlabel g (dst g e)).(block_mark) = true ->
+    let new_g := labeledgraph_gen_dst g e (vlabel g (dst g e)).(block_copied_vertex) in
+    forward_relation from to depth (inr e) g new_g
+| fr_e_to_not_forwarded_O: forall e (g: HeapGraph),
+    addr_gen (dst g e) = from -> (vlabel g (dst g e)).(block_mark) = false ->
+    let new_g := labeledgraph_gen_dst (lgraph_copy_v g (dst g e) to) e
+                                      (new_copied_v g to) in
+    forward_relation from to O (inr e) g new_g
+| fr_e_to_not_forwarded_Sn: forall depth e (g g': HeapGraph),
+    addr_gen (dst g e) = from -> (vlabel g (dst g e)).(block_mark) = false ->
+    let new_g := labeledgraph_gen_dst (lgraph_copy_v g (dst g e) to) e
+                                      (new_copied_v g to) in
+    forward_loop from to depth (vertex_pos_pairs new_g (new_copied_v g to)) new_g g' ->
+    forward_relation from to (S depth) (inr e) g g'
+with
+forward_loop (from to: nat): nat -> list forward_p_type -> HeapGraph -> HeapGraph -> Prop :=
+| fl_nil: forall depth g, forward_loop from to depth nil g g
+| fl_cons: forall depth g1 g2 g3 f fl,
+    forward_relation from to depth (forward_p2forward_t f nil g1) g1 g2 ->
+    forward_loop from to depth fl g2 g3 -> forward_loop from to depth (f :: fl) g1 g3.
+
+Lemma fr_general_prop_bootstrap: forall depth from to p g g'
+                                        (P: nat -> HeapGraph -> HeapGraph -> Prop),
+    (forall to g, P to g g) ->
+    (forall to g1 g2 g3, P to g1 g2 -> P to g2 g3 -> P to g1 g3) ->
+    (forall to g e v, P to g (labeledgraph_gen_dst g e v)) ->
+    (forall to g v, P to g (lgraph_copy_v g v to)) ->
+    forward_relation from to depth p g g' -> P to g g'.
+Proof.
+  induction depth; intros.
+  - inversion H3; subst; try (specialize (H to g'); assumption).
+    + apply H2.
+    + subst new_g. apply H1.
+    + subst new_g. remember (lgraph_copy_v g (dst g e) to) as g1.
+      remember (labeledgraph_gen_dst g1 e (new_copied_v g to)) as g2.
+      cut (P to g1 g2). 2: subst; apply H1. intros. apply (H0 to g g1 g2).
+      2: assumption. subst g1. apply H2.
+  - assert (forall l from to g1 g2,
+                 forward_loop from to depth l g1 g2 -> P to g1 g2). {
+    induction l; intros; inversion H4. 1: apply H. subst.
+    specialize (IHl _ _ _ _ H11). specialize (IHdepth _ _ _ _ _ _ H H0 H1 H2 H8).
+    apply (H0 _ _ _ _ IHdepth IHl). }
+    clear IHdepth. inversion H3; subst; try (specialize (H to g'); assumption).
+    + cut (P to g new_g).
+      * intros. apply (H0 to g new_g g'). 1: assumption. apply (H4 _ _ _ _ _ H8).
+      * subst new_g. apply H2.
+    + subst new_g. apply H1.
+    + cut (P to g new_g).
+      * intros. apply (H0 to g new_g g'). 1: assumption. apply (H4 _ _ _ _ _ H8).
+      * subst new_g. remember (lgraph_copy_v g (dst g e) to) as g1.
+        remember (labeledgraph_gen_dst g1 e (new_copied_v g to)) as g2.
+        cut (P to g1 g2). 2: subst; apply H1. intros. apply (H0 to g g1 g2).
+        2: assumption. subst g1. apply H2.
+Qed.
+
+Lemma fr_graph_has_gen: forall depth from to p g g',
+    graph_has_gen g to -> forward_relation from to depth p g g' ->
+    forall x, graph_has_gen g x <-> graph_has_gen g' x.
+Proof.
+  intros. remember (fun to g1 g2 =>
+                      graph_has_gen g1 to ->
+                      forall x, graph_has_gen g1 x <-> graph_has_gen g2 x) as P.
+  pose proof (fr_general_prop_bootstrap depth from to p g g' P). subst P.
+  apply H1; clear H1; intros; try assumption; try reflexivity.
+  - rewrite H1 by assumption. apply H2. rewrite <- H1; assumption.
+  - apply lcv_graph_has_gen. assumption.
+Qed.
+
+Lemma fl_graph_has_gen: forall from to depth l g g',
+    graph_has_gen g to -> forward_loop from to depth l g g' ->
+    forall x, graph_has_gen g x <-> graph_has_gen g' x.
+Proof.
+  intros. revert g g' H H0 x. induction l; intros; inversion H0. 1: reflexivity.
+  subst. assert (forall y, graph_has_gen g y <-> graph_has_gen g2 y) by
+      (intros; apply (fr_graph_has_gen _ _ _ _ _ _ H H4)).
+  transitivity (graph_has_gen g2 x). 1: apply H1. rewrite H1 in H.
+  apply IHl; assumption.
+Qed.
+
+Lemma fr_general_prop:
+  forall depth from to p g g' A (Q: HeapGraph -> A -> nat -> Prop)
+         (P: HeapGraph -> HeapGraph -> A -> Prop) (R: nat -> nat -> Prop),
+    R from to -> graph_has_gen g to -> (forall g v, P g g v) ->
+    (forall g1 g2 g3 v, P g1 g2 v -> P g2 g3 v -> P g1 g3 v) ->
+    (forall g e v x, P g (labeledgraph_gen_dst g e v) x) ->
+    (forall from g v to x,
+        graph_has_gen g to -> Q g x from -> (vlabel g v).(block_mark) = false ->
+        R from to -> addr_gen v = from -> P g (lgraph_copy_v g v to) x) ->
+    (forall depth from to p g g',
+        graph_has_gen g to -> forward_relation from to depth p g g' ->
+        forall v, Q g v from -> Q g' v from) ->
+    (forall g v to x from, graph_has_gen g to -> Q g x from ->
+                           Q (lgraph_copy_v g v to) x from) ->
+    (forall g e v x from, Q g x from -> Q (labeledgraph_gen_dst g e v) x from) ->
+    forward_relation from to depth p g g' ->
+    forall v, Q g v from -> P g g' v.
+Proof.
+  induction depth; intros.
+  - inversion H8; subst; try (specialize (H1 g' v); assumption).
+    + apply (H4 (addr_gen v0)); [assumption.. | reflexivity].
+    + subst new_g. apply H3.
+    + subst new_g. remember (lgraph_copy_v g (dst g e) to) as g1.
+      remember (labeledgraph_gen_dst g1 e (new_copied_v g to)) as g2.
+      cut (P g1 g2 v). 2: subst; apply H3. intros. apply (H2 g g1 g2).
+      2: assumption. subst g1.
+      apply (H4 (addr_gen (dst g e))); [assumption.. | reflexivity].
+  - assert (forall l from to g1 g2,
+               graph_has_gen g1 to -> forward_loop from to depth l g1 g2 ->
+               R from to -> forall v, Q g1 v from -> P g1 g2 v). {
+      induction l; intros; inversion H11. 1: apply H1. subst.
+      specialize (IHdepth _ _ _ _ _ _ _ _ _ H12 H10 H1 H2 H3 H4 H5 H6 H7 H17 _ H13).
+      apply (H5 _ _ _ _ _ _ H10 H17) in H13.
+      rewrite (fr_graph_has_gen _ _ _ _ _ _ H10 H17) in H10.
+      specialize (IHl _ _ _ _ H10 H20 H12 _ H13). apply (H2 _ _ _ _ IHdepth IHl). }
+    clear IHdepth. inversion H8; subst; try (specialize (H1 g' v); assumption).
+    + cut (P g new_g v).
+      * intros. apply (H2 g new_g g'). 1: assumption.
+        assert (graph_has_gen new_g to) by
+            (subst new_g; rewrite <- lcv_graph_has_gen; assumption).
+        apply (H10 _ _ _ _ _ H12 H14 H). subst new_g. apply H6; assumption.
+      * subst new_g. apply (H4 (addr_gen v0)); [assumption.. | reflexivity].
+    + subst new_g. apply H3.
+    + cut (P g new_g v).
+      * intros. apply (H2 g new_g g'). 1: assumption.
+        assert (graph_has_gen new_g to) by
+            (subst new_g; rewrite lgd_graph_has_gen, <- lcv_graph_has_gen; assumption).
+        apply (H10 _ _ _ _ _ H12 H14 H). subst new_g. apply H7, H6; assumption.
+      * subst new_g. remember (lgraph_copy_v g (dst g e) to) as g1.
+        remember (labeledgraph_gen_dst g1 e (new_copied_v g to)) as g2.
+        cut (P g1 g2 v). 2: subst; apply H3. intros. apply (H2 g g1 g2).
+        2: assumption. subst g1.
+        apply (H4 (addr_gen (dst g e))); [assumption.. | reflexivity].
+Qed.
+
+Lemma fr_graph_has_v: forall depth from to p g g',
+    graph_has_gen g to -> forward_relation from to depth p g g' ->
+    forall v, graph_has_v g v -> graph_has_v g' v.
+Proof.
+  intros. remember (fun (g: HeapGraph) (v: Addr) (x: nat) => True) as Q.
+  remember (fun g1 g2 v => graph_has_v g1 v -> graph_has_v g2 v) as P.
+  remember (fun (x1 x2: nat) => True) as R.
+  pose proof (fr_general_prop depth from to p g g' _ Q P R). subst Q P R.
+  apply H2; clear H2; intros; try assumption; try reflexivity.
+  - apply H3, H2. assumption.
+  - unfold lgraph_copy_v. rewrite <- lmc_graph_has_v.
+    apply lacv_graph_has_v_old; assumption.
+Qed.
+
+
+Lemma fr_gen_start: forall depth from to p g g',
+    graph_has_gen g to -> forward_relation from to depth p g g' ->
+    forall x, gen_start g x = gen_start g' x.
+Proof.
+  intros. remember (fun (g: HeapGraph) (v: nat) (x: nat) => True) as Q.
+  remember (fun g1 g2 x => gen_start g1 x = gen_start g2 x) as P.
+  remember (fun (x1 x2: nat) => True) as R.
+  pose proof (fr_general_prop depth from to p g g' _ Q P R). subst Q P R.
+  apply H1; clear H1; intros; try assumption; try reflexivity.
+  - rewrite H1. assumption.
+  - rewrite lcv_gen_start; [reflexivity | assumption].
+Qed.
+
+Lemma fl_gen_start: forall from to depth l g g',
+    graph_has_gen g to -> forward_loop from to depth l g g' ->
+    forall x, gen_start g x = gen_start g' x.
+Proof.
+  intros. revert g g' H H0 x. induction l; intros; inversion H0. 1: reflexivity.
+  subst. transitivity (gen_start g2 x).
+  - apply (fr_gen_start _ _ _ _ _ _ H H4).
+  - assert (graph_has_gen g2 to) by
+        (rewrite <- (fr_graph_has_gen _ _ _ _ _ _ H H4); assumption).
+    apply IHl; assumption.
+Qed.
+
+Lemma fr_vertex_size: forall depth from to p g1 g2,
+    graph_has_gen g1 to -> forward_relation from to depth p g1 g2 ->
+    forall v, graph_has_v g1 v -> vertex_size g1 v = vertex_size g2 v.
+Proof.
+  intros. remember (fun g v (x: nat) => graph_has_v g v) as Q.
+  remember (fun g1 g2 v => vertex_size g1 v = vertex_size g2 v) as P.
+  remember (fun (x1 x2: nat) => True) as R.
+  pose proof (fr_general_prop depth from to p g1 g2 _ Q P R). subst Q P R.
+  apply H2; clear H2; intros; try assumption; try reflexivity.
+  - rewrite H2. assumption.
+  - rewrite lcv_vertex_size_old; [reflexivity | assumption..].
+  - apply (fr_graph_has_v _ _ _ _ _ _ H2 H3 _ H4).
+  - apply lcv_graph_has_v_old; assumption.
+Qed.
+
+Lemma fr_O_nth_gen_unchanged: forall from to p g1 g2,
+    graph_has_gen g1 to -> forward_relation from to O p g1 g2 ->
+    forall gen, gen <> to -> nth_gen g1 gen = nth_gen g2 gen.
+Proof.
+  intros. inversion H0; subst; try reflexivity.
+  - rewrite lcv_nth_gen; auto.
+  - subst new_g. transitivity (nth_gen (lgraph_copy_v g1 (dst g1 e) to) gen).
+    2: reflexivity. rewrite lcv_nth_gen; [reflexivity | assumption..].
+Qed.
+
+Lemma fr_O_graph_gen_size_unchanged: forall from to p g1 g2,
+    graph_has_gen g1 to -> forward_relation from to O p g1 g2 ->
+    forall gen, graph_has_gen g1 gen -> gen <> to ->
+                graph_gen_size g1 gen = graph_gen_size g2 gen.
+Proof.
+  intros. unfold graph_gen_size.
+  erewrite <- (fr_O_nth_gen_unchanged from to _ g1 g2); eauto.
+  unfold previous_vertices_size. apply fold_left_ext. intros.
+  unfold vertex_size_accum. f_equal. rewrite nat_inc_list_In_iff in H3.
+  eapply (fr_vertex_size O from to); eauto. split; simpl; assumption.
+Qed.
+
+
+Definition forward_p_compatible
+           (p: forward_p_type) (roots: roots_t) (g: HeapGraph) (from: nat): Prop :=
+  match p with
+  | inl root_index => 0 <= root_index < Zlength roots
+  | inr (v, n) => graph_has_v g v /\ 0 <= n < Zlength (vlabel g v).(block_fields) /\
+                  (vlabel g v).(block_mark) = false /\ addr_gen v <> from
+  end.
+
+
+Definition upd_roots (from to: nat) (forward_p: forward_p_type)
+           (g: HeapGraph) (roots: roots_t) (f_info: fun_info): roots_t :=
+  match forward_p with
+  | inr _ => roots
+  | inl index => match Znth index roots with
+                 | inl (inl z) => roots
+                 | inl (inr p) => roots
+                 | inr v => if Nat.eq_dec (addr_gen v) from
+                            then if (vlabel g v).(block_mark)
+                                 then upd_bunch index f_info roots
+                                                (inr (vlabel g v).(block_copied_vertex))
+                                 else upd_bunch index f_info roots
+                                                (inr (new_copied_v g to))
+                            else roots
+                 end
+  end.
+
+Lemma upd_roots_Zlength: forall from to p g roots f_info,
+    Zlength roots = Zlength (live_roots_indices f_info) ->
+    Zlength (upd_roots from to p g roots f_info) = Zlength roots.
+Proof.
+  intros. unfold upd_roots. destruct p. 2: reflexivity.
+  destruct (Znth z roots). 1: destruct s; reflexivity. if_tac. 2: reflexivity.
+  destruct (block_mark (vlabel g a)); rewrite upd_bunch_Zlength; auto.
+Qed.
+
+
+Inductive forward_roots_loop (from to: nat) (f_info: fun_info):
+  list nat -> roots_t -> HeapGraph -> roots_t -> HeapGraph -> Prop :=
+| frl_nil: forall g roots, forward_roots_loop from to f_info nil roots g roots g
+| frl_cons: forall g1 g2 g3 i il roots1 roots3,
+    forward_relation from to O (root2forward (Znth (Z.of_nat i) roots1)) g1 g2 ->
+    forward_roots_loop from to f_info il
+                       (upd_roots from to (inl (Z.of_nat i)) g1 roots1 f_info)
+                       g2 roots3 g3 ->
+    forward_roots_loop from to f_info (i :: il) roots1 g1 roots3 g3.
+
+Definition forward_roots_relation from to f_info roots1 g1 roots2 g2 :=
+  forward_roots_loop from to f_info (nat_inc_list (length roots1)) roots1 g1 roots2 g2.
+
+
+Definition forward_condition g t_info from to: Prop :=
+  enough_space_to_copy g t_info from to /\
+  graph_has_gen g from /\ graph_has_gen g to /\
+  copy_compatible g /\ no_dangling_dst g.
