src/model/update.v
@@ -1,0 +1,124 @@
+From Coq Require Import Lists.List.
+
+From VST Require Import floyd.sublist.
+From VST Require Import veric.base.
+
+From CertiGraph Require Import graph.graph_model.
+From CertiGraph Require Import lib.List_ext.
+
+From CertiGC Require Import model.compatible.
+From CertiGC Require Import model.constants.
+From CertiGC Require Import model.graph.
+From CertiGC Require Import model.heap.
+From CertiGC Require Import model.thread_info.
+From CertiGC Require Import model.util.
+
+
+Definition upd_bunch (index: Z) (f_info: fun_info)
+           (roots: roots_t) (v: root_t): roots_t :=
+  fold_right (fun i rs => upd_Znth i rs v) roots
+             (get_indices index (live_roots_indices f_info)).
+
+Lemma upd_bunch_graph_compatible: forall g f_info roots z,
+    roots_graph_compatible roots g ->
+    forall v : Addr,
+      graph_has_v g v ->
+      roots_graph_compatible (upd_bunch z f_info roots (inr v)) g.
+Proof.
+  intros. red in H |-* . rewrite Forall_forall in H |-* . intros.
+  rewrite <- filter_sum_right_In_iff in H1. unfold upd_bunch in H1.
+  apply fold_right_upd_Znth_In in H1. destruct H1. 2: inversion H1; assumption.
+  apply H. rewrite <- filter_sum_right_In_iff. assumption.
+Qed.
+
+Lemma upd_bunch_Zlength: forall (f_info : fun_info) (roots : roots_t) (z : Z),
+    Zlength roots = Zlength (live_roots_indices f_info) ->
+    forall r : root_t, Zlength (upd_bunch z f_info roots r) = Zlength roots.
+Proof.
+  intros. unfold upd_bunch. apply fold_right_upd_Znth_Zlength.
+  intros. rewrite H. rewrite get_indices_spec in H0. destruct H0; assumption.
+Qed.
+
+Lemma upd_bunch_same: forall f_info roots z j r,
+    0 <= j < Zlength roots ->
+    Zlength roots = Zlength (live_roots_indices f_info) ->
+    Znth j (live_roots_indices f_info) = Znth z (live_roots_indices f_info) ->
+    Znth j (upd_bunch z f_info roots r) = r.
+Proof.
+  intros. unfold upd_bunch. apply fold_right_upd_Znth_same.
+  - intros. rewrite get_indices_spec in H2. destruct H2. rewrite H0; assumption.
+  - rewrite get_indices_spec. split; [rewrite <- H0|]; assumption.
+Qed.
+
+Lemma upd_bunch_diff: forall f_info roots z j r,
+    0 <= j < Zlength roots ->
+    Zlength roots = Zlength (live_roots_indices f_info) ->
+    Znth j (live_roots_indices f_info) <> Znth z (live_roots_indices f_info) ->
+    Znth j (upd_bunch z f_info roots r) = Znth j roots.
+Proof.
+  intros. unfold upd_bunch. apply fold_right_upd_Znth_diff. 3: assumption.
+  - intros. rewrite get_indices_spec in H2. destruct H2. rewrite H0; assumption.
+  - rewrite get_indices_spec. intro. destruct H2. apply H1. assumption.
+Qed.
+
+
+Lemma upd_thread_info_Zlength: forall (t: thread_info) (i: Z) (v: val),
+    0 <= i < MAX_ARGS -> Zlength (upd_Znth i (ti_args t) v) = MAX_ARGS.
+Proof.
+  intros. rewrite upd_Znth_Zlength; [apply arg_size | rewrite arg_size; assumption].
+Qed.
+
+Definition upd_thread_info_arg
+           (t: thread_info) (i: Z) (v: val) (H: 0 <= i < MAX_ARGS) : thread_info :=
+  Build_thread_info (ti_heap_p t) (ti_heap t) (upd_Znth i (ti_args t) v)
+                    (upd_thread_info_Zlength t i v H).
+
+Lemma upd_fun_thread_arg_compatible: forall g t_info f_info roots z,
+    fun_thread_arg_compatible g t_info f_info roots ->
+    forall (v : Addr) (HB : 0 <= Znth z (live_roots_indices f_info) < MAX_ARGS),
+      fun_thread_arg_compatible
+        g (upd_thread_info_arg t_info (Znth z (live_roots_indices f_info))
+                               (vertex_address g v) HB) f_info
+        (upd_bunch z f_info roots (inr v)).
+Proof.
+  intros. red in H |-* . unfold upd_thread_info_arg. simpl. rewrite Znth_list_eq in H.
+  destruct H. rewrite !Zlength_map in H. rewrite Zlength_map in H0.
+  assert (Zlength (upd_bunch z f_info roots (inr v)) = Zlength roots) by
+      (rewrite upd_bunch_Zlength; [reflexivity | assumption]).
+  rewrite Znth_list_eq. split. 1: rewrite !Zlength_map, H1; assumption. intros.
+  rewrite Zlength_map, H1 in H2.
+  rewrite !Znth_map; [|rewrite <- H | rewrite H1]; [|assumption..].
+  specialize (H0 _ H2). rewrite !Znth_map in H0; [|rewrite <- H| ]; [|assumption..].
+  destruct (Z.eq_dec (Znth j (live_roots_indices f_info))
+                     (Znth z (live_roots_indices f_info))).
+  - rewrite e, upd_Znth_same. 2: now rewrite arg_size.
+    rewrite upd_bunch_same; [|assumption..]. reflexivity.
+  - rewrite upd_Znth_diff. 4: assumption. 3: now rewrite arg_size.
+    + rewrite <- H0. rewrite upd_bunch_diff; [|assumption..]. reflexivity.
+    + rewrite arg_size. apply (fi_index_range f_info), Znth_In.
+      rewrite <- H. assumption.
+Qed.
+
+
+Lemma upd_roots_outlier_compatible: forall f_info roots outlier z v,
+    roots_outlier_compatible roots outlier ->
+    (* forall v : Addr, *)
+    (*   graph_has_v g v -> *)
+    roots_outlier_compatible (upd_bunch z f_info roots (inr v)) outlier.
+Proof.
+  intros. do 2 red in H |-* . intros.
+  rewrite <- filter_sum_right_In_iff, <- filter_sum_left_In_iff in H0.
+  unfold upd_bunch in H0. apply fold_right_upd_Znth_In in H0. destruct H0.
+  2: inversion H0. apply H.
+  rewrite <- filter_sum_right_In_iff, <- filter_sum_left_In_iff. assumption.
+Qed.
+
+Lemma upd_roots_compatible: forall g f_info roots outlier z,
+    roots_compatible g outlier roots ->
+    forall v : Addr, graph_has_v g v ->
+                      roots_compatible g outlier (upd_bunch z f_info roots (inr v)).
+Proof.
+  intros. destruct H. split.
+  - apply upd_roots_outlier_compatible; assumption.
+  - apply upd_bunch_graph_compatible; assumption.
+Qed.
